\documentclass{article}
\usepackage{amsmath} % for math symbols and environments

\begin{document}

The equation for horizontal motion in y-directoin is given by:
\begin{equation}
y(t) = \beta_{y, 1} e^{\alpha t} + \beta_{y, 2} e^{-\alpha t} + p_y(t)
\end{equation}
where
\begin{align*}
    \beta_{y, 1} &= \frac{(y_0 - p_{0, y})}{2} + \frac{\dot{y}_0 T - (p_{T, y} - p_{0, y})}{2 \alpha T}, \\
    \beta_{y, 2} &= \frac{(y_0 - p_{0, y})}{2} - \frac{\dot{y}_0 T - (p_{T, y} - p_{0, y})}{2 \alpha T}, \\
    \alpha &= \sqrt{\frac{g}{h}}.
\end{align*}

\end{document}
